Params change: this probably breaks correctness CI

proof/XMSS_Security_RFCAbs.ec
@@ -211,6 +211,9 @@ clone import XMSS_TW as XMSS_Security with
   op FLXMSSTW.n <- n,
   op FLXMSSTW.log2_w <- log2_w,
   op FLXMSSTW.w <- w,
+  op FLXMSSTW.len1 <- len1,
+  op FLXMSSTW.len2 <- len2,
+  op FLXMSSTW.len <- len,
   op FLXMSSTW.h <- h,
   op FLXMSSTW.chtype <= 0,
   op FLXMSSTW.pkcotype <= 1,
@@ -249,7 +252,7 @@ clone import XMSS_TW as XMSS_Security with
       let xl = take (8 * n) x in
       let xr = drop (8 * n) x in
       nb2db (rand_hash ps mad (NBytes.insubd (BitsToBytes xl)) (NBytes.insubd (BitsToBytes xr)))
-     else if i = 8 * n * Top.len then
+     else if i = 8 * n * len then
       let wpk = LenNBytes.insubd (map NBytes.insubd (chunk n (BitsToBytes x))) in
       nb2db (ltree ps mad wpk)
      else witness)
@@ -739,8 +742,7 @@ seq 1: (i = 0)=> //.
   + move=> ih.
     seq -1: (0 <= i <= Params.len)=> //.
     + wp; call Chain_chain_ll.
-       wp; auto=> />; smt(vals_w).
-       
+      by wp; auto=> />; smt(w_vals).
     by hoare; wp; conseq (: true)=> //; 1:smt().
   + wp; conseq (: true)=> //.
     + smt().
@@ -2529,10 +2531,10 @@ module WOTS_Encode = {
     var msg, csum, csum_32, len_2_bytes, csum_bytes, csum_base_w;
 
     (* Convert message to base w *)
-    msg <@ BaseW.base_w(NBytes.val M, len1);
+    msg <@ Top.BaseW.BaseW.base_w(m, len1);
 
     (* Compute checksum *)
-    csum <@ checksum(msg);
+    csum <@ WOTS.checksum(msg);
     csum_32 <- W32.of_int csum;
 
     (* Convert checksum to base w *)
@@ -2540,8 +2542,8 @@ module WOTS_Encode = {
     len_2_bytes <- ceil( ( len2 * log2_w )%r / 8%r );
 
     (* msg = msg || base_w(toByte(csum_32, len_2_bytes), w, len_2); *)
-    csum_bytes <- toByte csum_32 len2;
-    csum_base_w <@ BaseW.base_w(csum_bytes, len2);
+    csum_bytes <- toByte csum_32 len_2_bytes;
+    csum_base_w <@ Top.BaseW.BaseW.base_w(csum_bytes, len2);
     msg <- msg ++ csum_base_w;
 
     (* (* Convert message to base w *) *)
@@ -2578,7 +2580,6 @@ equiv kg_eq (O <: DSS_RFC.RO.POracle) :
     ={arg} ==> pkrel res{1}.`1 res{2}.`2 /\ skrel res{1}.`2 res{2}.`1 /\ to_uint res{2}.`1.`idx = 0.
 proof.
 have ? := h_g0; have ? := expr_gt0.
-
 proc.
 inline {1} keygen.
 inline{2} sample_randomness.
@@ -2792,29 +2793,29 @@ move => ???rr Hrr; do split.
 qed.
 *)
 
-lemma eq_len1s :
-  XMSS_Security.FLXMSSTW.len1 = Params.len1.
-proof.
-rewrite /len1 /w.
-by case: w_vals => -> /=; rewrite fromintM.
-qed.
+(* lemma eq_len1s : *)
+(*   XMSS_Security.FLXMSSTW.len1 = Params.len1. *)
+(* proof. *)
+(* rewrite /len1 /w. *)
+(* by case: w_vals => -> /=; rewrite fromintM. *)
+(* qed. *)
 
 
-lemma eq_len2s :
-  XMSS_Security.FLXMSSTW.len2 = Params.len2.
-proof.
-rewrite /len2 /len1 /w.
-by case: w_vals => -> /=; rewrite ?fromintM.
-qed.
+(* lemma eq_len2s : *)
+(*   XMSS_Security.FLXMSSTW.len2 = Params.len2. *)
+(* proof. *)
+(* rewrite /len2 /len1 /w. *)
+(* by case: w_vals => -> /=; rewrite ?fromintM. *)
+(* qed. *)
 
 
-lemma eq_lens :
-  XMSS_Security.FLXMSSTW.len = Params.len.
-proof. by rewrite /len eq_len1s eq_len2s. qed.
+(* lemma eq_lens : *)
+(*   XMSS_Security.FLXMSSTW.len = Params.len. *)
+(* proof. by rewrite /len eq_len1s eq_len2s. qed. *)
 
 equiv sig_eq (O <: DSS_RFC.RO.POracle) _idx :
   XMSS_TW_RFC(O).sign ~ XMSS_RFC_Abs(RFC_O(O)).sign :
-  ={glob O} /\ skrel sk{1} sk{2} /\ ={m} /\ to_uint sk{2}.`idx = _idx /\ _idx <= 2^h - 1  ==>
+  ={glob O} /\ skrel sk{1} sk{2} /\ ={m} /\ to_uint sk{2}.`idx = _idx /\ _idx <= 2^h - 1 ==>
   ={glob O} /\  sigrel res{1}.`1 res{2}.`1 /\ to_uint res{2}.`2.`idx = _idx+1 /\ (_idx < 2^h - 1 => skrel res{1}.`2 res{2}.`2).
 proof.
 proc.
@@ -2975,9 +2976,9 @@ seq 1 1 : (   #pre
          /\ (forall j, 0 <= j < size sig2{1} =>
              nth witness sig2{1} j = bs2block (nth witness sig0{2} j))
          /\ size sig2{1} = i{2}
-         /\ size sig0{2} = Params.len
-         /\ size sig2{1} <= XMSS_Security.FLXMSSTW.len
-         /\ 0 <= i{2} <= Params.len).
+         /\ size sig0{2} = len
+         /\ size sig2{1} <= len
+         /\ 0 <= i{2} <= len).
   + wp.
     inline{2} chain; wp; sp => /=; elim*=> adrn.
     exlim address2{2}, t0{2} => ad2t t02t.
@@ -2988,9 +2989,9 @@ seq 1 1 : (   #pre
               /\ address2{2} = set_hash_addr ad2t (if chain_count{2} = 0 then 0 else chain_count{2} - 1)
               /\ ad2t = (set_chain_addr (set_ots_addr zero_address (to_uint idx0{2})) i{2})
               /\ 0 <= chain_count{2} <= s{2}
-              /\ 0 <= s{2} < Top.XMSS_Security.FLXMSSTW.w - 1
+              /\ 0 <= s{2} < w - 1
               /\ i0{2} = 0
-              /\ i{2} < Params.len)
+              /\ i{2} < len)
              (s{2} - chain_count{2}).
     + auto => &2 /> ih ge0_cc lts_cc *.
       do ? split; 3..:smt(w_vals).
@@ -3009,7 +3010,8 @@ seq 1 1 : (   #pre
           rewrite /BytesToBits (: n = size (map W8.w2bits (NBytes.val ft))).
           + by rewrite size_map NBytes.valP.
           by rewrite (size_flatten_ctt 8) => // bs /mapP [x] ->; rewrite size_w2bits.
-        do ? congr. admit.
+        do ? congr.
+        admit.
       rewrite /set_hash_addr ?setE /=; congr; rewrite fun_ext => i.
       case (i = 6) => [// /#| ?].
       rewrite initE /=.
@@ -3053,8 +3055,8 @@ seq 1 1 : (   #pre
     by rewrite size_rcons /#.
     smt(size_ge0).
     smt(size_ge0).
-    smt(size_rcons eq_lens).
-    smt(size_rcons eq_lens).
+    smt(size_rcons).
+    smt(size_rcons).
   wp -1 -1.
   sp; seq 1 1 : (#pre /\ DBLL.val skWOTS0{1} = map bs2block (LenNBytes.val wots_skey{2})).
   + admit.
@@ -3072,7 +3074,7 @@ seq 1 1 : (   #pre
   rewrite ?initE rngi /=.
   case (i = 4) => [// | nfr /=].
   case (i = 7) => [// | nfs /=].
-  smt(initE). 
+  smt(initE).
   rewrite /RFC.skr2sko /= zeroidxsE XAddress.insubdK.
   + by rewrite /valid_xadrs HAX.Adrs.insubdK 1:zeroadiP zeroxadiP.
   rewrite /set_typeidx /set_kpidx HAX.Adrs.insubdK /put /= 1:zeroadiP.
@@ -3087,25 +3089,22 @@ seq 1 1 : (   #pre
   rewrite nth_sub. smt(size_rev size_map size_sub).
   do ? (rewrite initE /=). pose t := size _.
   smt(size_rev size_map size_sub W32.initE W32.to_uintK_small W32.to_uint0 Index.valP ge1_h).
-  rewrite eq_len1s eq_len2s.
   rewrite /bs2block DigestBlock.insubdK /BytesToBits.
   rewrite (: n = size (map W8.w2bits (NBytes.val _M'{2}))) 1:size_map 1:NBytes.valP 1://.
   by rewrite (size_flatten_ctt 8) => // bs /mapP [x] ->; rewrite size_w2bits.
   rewrite -/EmsgWOTS.ofemsgWOTS EmsgWOTS.ofemsgWOTSK //.
   rewrite /encode_int size_cat /checksum /int2lbw /= ?size_mkseq.
-  smt(eq_len1s eq_len2s ge1_len1 ge1_len2).
+  smt(ge1_len1 ge1_len2).
   smt().
   rewrite size_nseq. smt(ge0_len).
   smt(ge2_len).
   smt(Params.ge0_len).
-  by smt(eq_lens).
-  smt(ge2_len).
   rewrite LenNBytes.insubdK. smt().
   congr; apply (eq_from_nth witness).
   smt(size_map). move=> i rngi.
   by rewrite (nth_map witness); smt().
 auto => &1 &2 /> ? eqv *.
-do split;last first. 
+do split;last first.
 + move => *; rewrite Index.insubdK; 1:smt(Index.valP).
 by rewrite /RFC.skr2sko /= eqv /= to_uintD_small; smt(pow2_32 expr_ge0 h_max gt_exprsbde h_g0).
 by rewrite /RFC.skr2sko /= eqv /=; smt(pow2_32 expr_ge0 h_max gt_exprsbde h_g0).
@@ -3267,7 +3266,7 @@ seq 5 9 : (   pkrel pk{1} pk{2}
     admit.
   move=> *.
   do ? split; 1: smt(Index.valP).
-  + rewrite eqs22 DBLL.insubdK 1:size_map 1:LenNBytes.valP; 1: smt(eq_lens).
+  + rewrite eqs22 DBLL.insubdK 1:size_map 1:LenNBytes.valP 1://.
     rewrite -map_comp /(\o) -eq_in_map => x /=; rewrite DigestBlock.insubdK 2://.
     rewrite (size_flatten_ctt 8); 1: by move=> y /mapP [t] ->; rewrite size_w2bits.
     by rewrite size_map NBytes.valP.
@@ -3285,6 +3284,8 @@ wp; inline{1} verify; inline{1} root_from_sigFLXMSSTW; inline{2} rootFromSig.
 sp; seq 1 1 : (   #pre
                /\ map DigestBlock.val (DBLL.val pkWOTS0{1}) = map (BytesToBits \o NBytes.val) (LenNBytes.val pk_ots{2})).
 + inline{1} pkWOTS_from_sigWOTS; inline{2} pkFromSig.
+  sp 4 5.
+  outline{2} [1 .. 8] by { msg <@ WOTS_Encode.encode(NBytes.val M0); }.
   admit.
 wp; sp 0 5; elim* => ad2.
 exlim nodes0{2} => lf2.
@@ -3396,7 +3397,7 @@ congr.
   rewrite (eq_map (_ \o (_ \o NBytes.val)) NBytes.val); 1: smt(BytesToBitsK).
   move => <-; rewrite LenNBytes.insubdK 1:size_map 1:size_chunk; 1: smt(ge1_n).
   + rewrite size_map size_chunk 1:// (size_flatten_ctt (8 * n)); 1: by move=> y /mapP [t] ->; rewrite DigestBlock.valP.
-    by rewrite size_map DBLL.valP mulzA ?mulKz 1://; smt(ge1_n eq_lens).
+    by rewrite size_map DBLL.valP mulzA ?mulKz 1://; smt(ge1_n).
   rewrite -map_comp; pose chn := chunk _ _.
   move/iffLR: (eq_in_map (NBytes.val \o NBytes.insubd) idfun chn) => /(_ _).
   + move => x /mapP [y] @/idfun /= [/mem_iota [ge lt] ->] @/(\o); rewrite NBytes.insubdK 2://.
@@ -3486,7 +3487,6 @@ conseq (_: _ ==> DigestBlock.val root'{1} = BytesToBits (NBytes.val nodes0{2})).
   move=> r0 r1 eqrs.
   rewrite -DigestBlock.valKd eqrs eqpk1.
   admit.
-  
 inline{1} root_from_sigFLXMSSTW.
 seq 14 11 : (   to_uint idx_sig0{2} < l
              /\ ps0{1} = _seed0{2}
@@ -3503,7 +3503,7 @@ seq 1 3 : (   to_uint idx_sig0{2} < l
            /\ (DBHL.val ap{1}) = map bs2block (AuthPath.val auth0{2})).
 wp.
 have ltree_ll : islossless LTree.ltree by admit.
-exlim pk_ots{2}, address0{2}, _seed0{2} => pkots2 add02 sd02. 
+exlim pk_ots{2}, address0{2}, _seed0{2} => pkots2 add02 sd02.
 call{2} (_: arg = (pkots2, add02, sd02) ==> res = ltree  sd02 add02 pkots2).  print Eqv_Ltree_ltree.
 by conseq ltree_ll (ltree_eq sd02 add02 pkots2).
 skip => &1 &2 /> ltlidx eqpkots eqidx eqap.
